Simple networking and saml stubs added

FSharpNemlogIn/FStarWrapper/Program.fs
@@ -1,9 +1,14 @@
-﻿// Learn more about F# at http://fsharp.net
-// See the 'F# Tutorial' project for more help.
-open System
+﻿open System
+open Network
+
 [<EntryPoint>]
 let main argv = 
 //    print.printf_fst (Array.get argv 0)
-    Main.main "thesp" "theuri" "me" "myPassword"
+    //Main.main "thesp" "theuri" "me" "myPassword"
+    let msg = X.GetReq "sp" "idp"
+    printfn "%s" msg
+
+    let _ = X.CreateSendAndRecieve "sp" "idp"
+   
     let key = Console.Read ()
     0 // return an integer exit code
