FSharpNemlogIn/Netw/Network.fs
@@ -1,0 +1,16 @@
+﻿module Network
+
+let fo param = 
+    param |> List.fold (fun r s -> r+ ";" + s) ""
+    
+
+let SendX (prin:string) (methodId:string)  (query:string) (cookies:string) (msg:string) = 
+//    let q = fo query
+//    let c = fo cookies
+    printfn "Message sent to: %s on %s with payload: %s and query:%s and Cookies:%s" prin methodId msg query cookies
+    Protocol.Success() :> Protocol.SamlStatus
+
+let RecieveX (prin:string) =
+    "Sending response:" + "I have recieved your request and this is my response" + " to: " +  prin
+    
+
