Protocol/print.fs
@@ -1,4 +1,0 @@
-﻿[<EntryPoint>]
-let main argv = 
-    print.printf_fst (Array.get argv 0)
-    0 // return an integer exit code
