Protocol/identityprovider.fst
@@ -6,34 +6,38 @@ val identityprovider: me:prin -> pubkey me -> privkey me
                       -> unit
 let identityprovider me pubk privk browser serviceprovider pubksp =
 	
-  let samlreq = recieve browser in (*3*)
+  let samlreq = Recieve browser in (*3*)
 	match samlreq with
 	| SamlProtocolMessage (idp, msg, sigSP)->  
 
-    if verify serviceprovider pubksp msg sigSP
+    if VerifySignature serviceprovider pubksp msg sigSP
     then
      (assert (Log serviceprovider msg);
-        let challenge = createChallenge browser in
-    
-        let challengeMessage = ChallengeMessage challenge in
-        send browser challengeMessage; (*4*)
-        let credentials = recieve browser in (*5*)
-        match credentials with
-          | Credentials(user, password, challenge') -> 
+      let challenge = CreateChallenge browser in
   
-          (*Check credentials and challenge*)
-  
-          let samlresponse = createSamlResponse me serviceprovider Success in
+      let challengeMessage = ChallengeMessage challenge in
+      Send browser challengeMessage; (*4*)
+      let credentials = Recieve browser in (*5*)
+      match credentials with
+        | Credentials(user, password, challenge') -> 
+
+        (*Check credentials and challenge*)
+        if AuthenticateUser user password challenge'
+        then
+          (assert (Log2 user password challenge');
+
+          let samlresponse = CreateSamlResponse me serviceprovider Success in
           assume(Log me samlresponse);
-          let sigIDP = sign me privk samlresponse in 
+          let sigIDP = Sign me privk samlresponse in 
           let response = SamlProtocolMessage serviceprovider samlresponse sigIDP in
-          send browser response(*6*)
+          Send browser response(*6*))
+        else Send browser (Failed (400))
   
-        | _ -> send browser (Failed (400)))(*6.3*)
-    else send browser (Failed (400))
+        | _ -> Send browser (Failed (400)))(*6.3*)
+    else Send browser (Failed (400))
   | _ -> 
-     let samlresponse = createSamlResponse me serviceprovider Requester in
+     let samlresponse = CreateSamlResponse me serviceprovider Requester in
      assume(Log me samlresponse);
-     let sigIDP = sign me privk samlresponse in
+     let sigIDP = Sign me privk samlresponse in
      let response = SamlProtocolMessage serviceprovider samlresponse sigIDP in
-     send browser response (*4.1*)
+     Send browser response (*4.1*)
