Protocol/FstNetwork.fst
@@ -1,0 +1,15 @@
+module FstNetwork
+open Protocol
+
+type method = string
+type queryparams = string
+type cookies = string
+type messagebody = string
+
+extern reference Network {language="F#";
+						dll="Network";
+						namespace="";
+						classname="Network"}
+extern Network val SendX: prin -> method -> queryparams -> cookies -> messagebody -> SamlStatus
+extern Network val RecieveX: prin -> string 
+extern Network val CreateSamlProtocolMessage: samlmessage -> dsig -> string
