Protocol/ModelUtil.fst
@@ -1,0 +1,3 @@
+module ModelUtil
+
+val Fork: list (unit -> unit) -> unit
