Protocol/ServiceProvider.fst
@@ -4,27 +4,27 @@ open Protocol
 val serviceprovider:  me:prin -> pubkey me -> privkey me ->
                       browser:prin -> idp:prin -> pubkey idp -> unit 
 let serviceprovider me pubk privk browser idp pubkidp = 
-  let reqRes = recieve browser in (*1*)
+  let reqRes = Recieve browser in (*1*)
   match reqRes with
   | HttpGet (uri) -> 
   
-    let authnReq = createAuthnRequest me idp in 
+    let authnReq = CreateAuthnRequest me idp in 
     assume(Log me authnReq) (*Protocol event*);
-    let sigSP = sign me privk authnReq in
+    let sigSP = Sign me privk authnReq in
       
     let authnReqest = SamlProtocolMessage idp authnReq sigSP in 
-    send browser authnReqest; (*2*)  
-    let authResponse = recieve browser in (*7*)
+    Send browser authnReqest; (*2*)  
+    let authResponse = Recieve browser in (*7*)
     match authResponse with
     | SamlProtocolMessage (sp, msg, sigIDP) -> 
-      (if verify idp pubkidp msg sigIDP
+      (if VerifySignature idp pubkidp msg sigIDP
       then
         (assert(Log idp msg);
           let resource = Resource uri in
-          send browser resource)  (*8*)
+          Send browser resource)  (*8*)
       else ())
-    | _ ->  send browser (Failed (403))(*8.1*)     
+    | _ ->  Send browser (Failed (403))(*8.1*)     
   
-  | _ -> send browser (Failed (400))(*2.1*)
+  | _ -> Send browser (Failed (400))(*2.1*)
 
 end (* Serviceprovider *)
