Protocol/X.fst
@@ -1,0 +1,29 @@
+module X
+
+open Protocol
+open FstNetwork
+
+val GetReq: prin -> prin -> samlmessage
+let GetReq sp idp = 
+	CreateAuthnRequest sp idp
+
+val CreateAndSend: prin -> prin ->unit
+let CreateAndSend sp idp =
+	let authReq = CreateAuthnRequest sp idp in
+	let req = SamlProtocolMessage sp authReq "sig" in
+	let status = SendX sp "GET" "query=Somevalue" "cookei=somevalue" "body" in
+	match status with
+	| Success -> print_string "great!";()
+	| _ -> print_string "crap!";()
+
+	
+val CreateSendAndRecieve: prin -> prin ->unit
+let CreateSendAndRecieve sp idp =
+	let authReq = CreateAuthnRequest sp idp in
+	let req = SamlProtocolMessage sp authReq "sig" in
+	let status = SendX sp "GET" "query=Somevalue" "cookei=somevalue" "body" in
+	match status with
+	| Success -> print_string "great!";
+		let resp = RecieveX sp in 
+			print_string resp; ()
+	| _ -> print_string "crap!";()
