Protocol/browser.fst
@@ -5,23 +5,23 @@ val browser: sp:prin -> res:uri -> user:string -> password:string -> unit
 let browser sp resource user password = 
     print_string "Entering Client (sending request)";
     let req = HttpGet resource in
-    let _ = send sp req in(*1*)
-      let res = recieve sp in(*2*)
+    let _ = Send sp req in(*1*)
+      let res = Recieve sp in(*2*)
         match res with
         | SamlProtocolMessage (idp, authnRequest, sigSP) -> 
           let samlAuthnReq = SamlProtocolMessage idp authnRequest sigSP in
-          send idp samlAuthnReq;
-          let chal = recieve idp in (*4*)
+          Send idp samlAuthnReq;
+          let chal = Recieve idp in (*4*)
           match chal with
           | ChallengeMessage (challenge) -> 
             let authUserReq = Credentials user password challenge in (*5*)
-            send idp authUserReq; (*5*)
-            let idpResp = recieve idp in
+            Send idp authUserReq; (*5*)
+            let idpResp = Recieve idp in
             match idpResp with
             | SamlProtocolMessage (sp', samlResponse, sigIDP) -> 
               let samlResponseRequest =  SamlProtocolMessage sp' samlResponse sigIDP in (*7*)
-              send sp' samlResponseRequest;
-              recieve sp'; () (*8*)
+              Send sp' samlResponseRequest;
+              Recieve sp'; () (*8*)
             | _ -> idpResp; () (*Report response back to caller*)
           | _ -> chal; () (*Report response back to caller*)
         | _ -> res; () (*Report response back to caller*)
