Protocol/main.fst
@@ -4,11 +4,12 @@ open Protocol
 open Browser
 open Serviceprovider
 open Identityprovider
+open ModelUtil
 
 let main attacker =
-	let sppk, spsk = keygen "https://serviceprovider.org" in 
-	let idppk, idpsk = keygen "https://identityprovider.org" in 
-	fork [	attacker;
+	let sppk, spsk = Keygen "https://serviceprovider.org" in 
+	let idppk, idpsk = Keygen "https://identityprovider.org" in 
+	Fork [	attacker;
 		(fun () -> browser "browser" "https://serviceprovider.org/protectedresource" "me" "myPassword");
 		(fun () -> serviceprovider "https://serviceprovider.org" sppk spsk "browser" "https://identityprovider.org" idppk);
 		(fun () -> identityprovider "https://identityprovider.org" idppk idpsk "browser" "https://serviceprovider.org" sppk)]
