Protocol/print.fst
@@ -1,6 +1,0 @@
-module print
-  val printf_fst : string -> unit
-  let printf_fst (string) =
-	 print_string string; ()
-
-end
