Saml/Script.fsx
@@ -1,0 +1,17 @@
+﻿// Learn more about F# at http://fsharp.net. See the 'F# Tutorial' project
+// for more guidance on F# programming.
+
+#load "Saml.fs"
+open Saml
+
+let authnReq = CreateAuthnRequest "mSp" "someIdp"
+printfn "%s"authnReq
+
+let challenge = CreateChallenge "prin"
+printfn "%s" challenge
+
+let resp = CreateSamlResponse "idp" "sp" "Success"
+printfn "%s" resp
+
+// Define your library scripting code here
+
